UPPAAL_Model_Checking.thy
@@ -1,0 +1,882 @@
+theory UPPAAL_Model_Checking
+  imports
+    UPPAAL_State_Networks_Impl_Refine
+    "~~/src/HOL/Library/BNF_Corec"
+begin
+
+hide_const models
+
+term "A \<turnstile>' \<langle>l, u\<rangle> \<rightarrow> \<langle>l', u'\<rangle>"
+
+term "Graph_Defs.Alw_ev (\<lambda> (l, u) (l', u'). A \<turnstile>' \<langle>l, u\<rangle> \<rightarrow> \<langle>l', u'\<rangle>)"
+
+term check_bexp
+
+definition models ("_,_ \<Turnstile>\<^sub>_ _" [61,61] 61) where
+  "A,a\<^sub>0 \<Turnstile>\<^sub>n \<Phi> \<equiv> (case \<Phi> of
+    formula.EX \<phi> \<Rightarrow>
+      Graph_Defs.Ex_ev
+        (\<lambda> (L, s, u) (L', s', u'). A \<turnstile>\<^sub>n \<langle>L, s, u\<rangle> \<rightarrow> \<langle>L', s', u'\<rangle>)
+        (\<lambda> (L, s, _). check_bexp \<phi> L s)
+  | formula.EG \<phi> \<Rightarrow>
+      Graph_Defs.Ex_alw
+        (\<lambda> (L, s, u) (L', s', u'). A \<turnstile>\<^sub>n \<langle>L, s, u\<rangle> \<rightarrow> \<langle>L', s', u'\<rangle>)
+        (\<lambda> (L, s, _). check_bexp \<phi> L s)
+  | formula.AX \<phi> \<Rightarrow>
+      Graph_Defs.Alw_ev
+        (\<lambda> (L, s, u) (L', s', u'). A \<turnstile>\<^sub>n \<langle>L, s, u\<rangle> \<rightarrow> \<langle>L', s', u'\<rangle>)
+        (\<lambda> (L, s, _). check_bexp \<phi> L s)
+  | formula.AG \<phi> \<Rightarrow>
+      Graph_Defs.Alw_alw
+        (\<lambda> (L, s, u) (L', s', u'). A \<turnstile>\<^sub>n \<langle>L, s, u\<rangle> \<rightarrow> \<langle>L', s', u'\<rangle>)
+        (\<lambda> (L, s, _). check_bexp \<phi> L s)
+  | formula.Leadsto \<phi> \<psi> \<Rightarrow>
+      Graph_Defs.leadsto
+        (\<lambda> (L, s, u) (L', s', u'). A \<turnstile>\<^sub>n \<langle>L, s, u\<rangle> \<rightarrow> \<langle>L', s', u'\<rangle>)
+        (\<lambda> (L, s, _). check_bexp \<phi> L s)
+        (\<lambda> (L, s, _). check_bexp \<psi> L s)
+  ) a\<^sub>0
+  "
+
+term "A,a\<^sub>0 \<Turnstile>\<^sub>n \<Phi>"
+
+lemmas models_iff = models_def[unfolded Graph_Defs.Ex_alw_iff Graph_Defs.Alw_alw_iff]
+
+term sscan term "\<lambda> xs. sscan (\<lambda> a (_, i). (a, Suc i)) xs (undefined, 0)"
+
+definition substream :: "'a stream => nat set => 'a stream" where
+"substream xs I =
+  smap fst (sfilter (\<lambda> (a, i). i \<in> I) (sscan (\<lambda> a (_, i). (a, Suc i)) xs (undefined, 0)))"
+
+lemma substream_eq_ConsD:
+  assumes "substream xs I = x ## as"
+  shows
+    "\<exists> ys zs.
+      xs = ys @- x ## zs \<and> length ys \<in> I \<and> (\<forall> i \<in> I. i \<ge> length ys)
+      \<and> substream zs ({i - length ys - 1 | i. i \<in> I \<and> i > length ys}) = as"
+    sorry
+
+lemma
+  "ev (holds P) xs" if "ev (holds P) (substream xs I)"
+  using that thm ev.induct
+  apply (induction "substream xs I" arbitrary: xs I)
+   apply simp
+  subgoal for xs I
+    apply (cases "substream xs I")
+    apply simp
+    apply (frule substream_eq_ConsD)
+    apply auto
+      oops
+
+context
+  fixes A :: "('a, 'c, 't :: time, 's) ta"
+begin
+
+interpretation G: Graph_Defs "\<lambda> (l, u) (l', u'). A \<turnstile> \<langle>l, u\<rangle> \<rightarrow> \<langle>l', u'\<rangle>" .
+interpretation G': Graph_Defs "\<lambda> (l, u) (l', u'). A \<turnstile>' \<langle>l, u\<rangle> \<rightarrow> \<langle>l', u'\<rangle>" .
+
+corec expand_run :: "('s \<times> ('c, 't) cval) stream \<Rightarrow> ('s \<times> ('c, 't) cval) stream" where
+  "expand_run xs =
+    (case xs of (l, u) ## (l', u') ## ys \<Rightarrow>
+      (l, u) ## (l, SOME u''. \<exists> a d. A \<turnstile> \<langle>l, u\<rangle> \<rightarrow>\<^bsup>d\<^esup> \<langle>l, u''\<rangle> \<and> A \<turnstile> \<langle>l, u''\<rangle> \<rightarrow>\<^bsub>a\<^esub> \<langle>l', u'\<rangle>)
+      ## expand_run ((l', u') ## ys)
+    )"
+
+lemma
+  "\<exists> xs. G.run (x ## xs) \<and> alw (holds (\<lambda> (l, u). P l)) (x ## xs)"
+  if "G'.run (x ## xs)" "alw (holds (\<lambda> (l, u). P l)) (x ## xs)"
+proof -
+  from that(1) have "G.run (expand_run (x ## xs))"
+  proof (coinduction arbitrary: x xs)
+    case run
+    then show ?case sorry -- "Need to proof specialized coinduction rule for G.rule"
+  qed
+oops
+
+end
+
+
+(* XXX Move *)
+lemma cval_add_0:
+  "u \<oplus> 0 = u" for u :: "(_, _ :: time) cval"
+  unfolding cval_add_def by simp
+
+lemma Ex_ev_eq_reachability:
+  assumes
+    "\<forall>p<length (fst (snd A)). \<exists>pc st s' rs.
+       stepst (fst A) n u
+          ((fst (snd (snd A)) ! p) (L ! p), [], s, True, [])
+          (pc, st, s', True, rs)"
+    "\<forall>p<length (fst (snd A)). u \<turnstile> snd (fst (snd A) ! p) (L ! p)"
+    "bounded (snd (snd (snd A))) s"
+  shows
+  "Graph_Defs.Ex_ev
+    (\<lambda> (L, s, u) (L', s', u'). A \<turnstile>\<^sub>n \<langle>L, s, u\<rangle> \<rightarrow> \<langle>L', s', u'\<rangle>)
+    (\<lambda> (L, s, _). P L s) (L, s, u)
+   \<longleftrightarrow> (\<exists> L' s' u'. A \<turnstile>\<^sub>n \<langle>L, s, u\<rangle> \<rightarrow>* \<langle>L', s', u'\<rangle> \<and> P L' s')
+  "
+  unfolding Graph_Defs.Ex_ev_def
+  apply safe
+  subgoal for xs
+    apply (drule ev_imp_shift)
+    apply safe
+    subgoal for ys zs
+      apply (cases zs)
+      apply clarsimp
+      subgoal premises prems for L' s' u' ws
+        proof (cases ys)
+          case Nil
+          with prems show ?thesis
+            by fastforce
+        next
+          case (Cons a us)
+          with prems have
+            "Graph_Defs.run (\<lambda>(L, s, u) (L', x, y). A \<turnstile>\<^sub>n \<langle>L, s, u\<rangle> \<rightarrow> \<langle>L', x, y\<rangle>)
+              ((L, s, u) ## us @- (L', s', u') ## ws)"
+            by simp
+          with \<open>P _ _\<close> show ?thesis
+          proof (induction us arbitrary: L s u)
+            case Nil
+            then show ?case
+              apply (inst_existentials L' s')
+              apply clarsimp
+              apply (erule Graph_Defs.run.cases)
+              apply clarify
+              apply (inst_existentials u')
+              apply rule
+              by auto
+          next
+            case (Cons a us)
+            obtain L'' s'' u'' where [simp]: "a = (L'', s'', u'')"
+              by (cases a) auto
+            from Cons.prems(2) Cons.IH[OF \<open>P _ _\<close>] obtain L' s' a where
+              "A \<turnstile>\<^sub>n \<langle>L'', s'', u''\<rangle> \<rightarrow>* \<langle>L', s', a\<rangle>" "P L' s'"
+              by atomize_elim (fastforce elim: Graph_Defs.run.cases)
+            with Cons.prems(2) show ?case
+              by - (erule Graph_Defs.run.cases, clarsimp, metis stepI2)
+          qed
+        qed
+        done
+      done
+    subgoal premises prems for L' s' u'
+    proof -
+      interpret Graph_Defs "\<lambda>(L, s, u) (L', x, y). A \<turnstile>\<^sub>n \<langle>L, s, u\<rangle> \<rightarrow> \<langle>L', x, y\<rangle>" .
+      from prems(1) have "reaches (L, s, u) (L', s', u')"
+        by (induction; blast intro!: rtranclp.rtrancl_into_rtrancl)
+      from reaches_steps[OF this] guess xs by clarify
+      note xs = this
+      from prems(1) have "A \<turnstile>\<^sub>n \<langle>L', s', u'\<rangle> \<rightarrow> \<langle>L', s', u' \<oplus> 0\<rangle>"
+        apply cases
+        subgoal
+          using assms by (cases A)  (simp add: , rule step_u_t, auto simp: cval_add_0)
+        subgoal
+          by (cases A, simp, rule step_u_t, auto simp: cval_add_0 elim!: step_u.cases)
+        done
+      then have "run (sconst (L', s', u'))"
+        by coinduction (simp add: cval_add_0)
+      with xs have "run (xs @- sconst (L', s', u'))"
+        by - (subst siterate.ctr, erule run.cases, clarsimp, rule extend_run, auto)
+      with xs \<open>P _ _\<close> show ?thesis
+        apply (inst_existentials "tl xs @- sconst (L', s', u')")
+        subgoal
+          by (erule steps.cases; simp)
+        subgoal
+          apply (erule steps.cases)
+           apply (simp, rule ev.base, simp; fail)
+          apply (subst append_butlast_last_id[of xs, symmetric])
+           apply (simp; fail)
+          apply (fastforce intro: ev_shift)
+          done
+        done
+    qed
+    done
+
+lemma models_alt_def:
+  assumes
+    "\<forall>p<length (fst (snd A)). \<exists>pc st s' rs.
+       stepst (fst A) n u
+          ((fst (snd (snd A)) ! p) (L ! p), [], s, True, [])
+          (pc, st, s', True, rs)"
+    "\<forall>p<length (fst (snd A)). u \<turnstile> snd (fst (snd A) ! p) (L ! p)"
+    "bounded (snd (snd (snd A))) s"
+  shows
+    "A,(L,s,u) \<Turnstile>\<^sub>n \<Phi> = (case \<Phi> of
+      formula.EX \<phi> \<Rightarrow>
+        (\<lambda> (L, s, u). \<exists> L' s' u'. A \<turnstile>\<^sub>n \<langle>L, s, u\<rangle> \<rightarrow>* \<langle>L', s', u'\<rangle> \<and> check_bexp \<phi> L' s')
+    | formula.EG \<phi> \<Rightarrow>
+        Not o Graph_Defs.Alw_ev
+          (\<lambda> (L, s, u) (L', s', u'). A \<turnstile>\<^sub>n \<langle>L, s, u\<rangle> \<rightarrow> \<langle>L', s', u'\<rangle>)
+          (\<lambda> (L, s, _). \<not> check_bexp \<phi> L s)
+    | formula.AX \<phi> \<Rightarrow>
+        Graph_Defs.Alw_ev
+          (\<lambda> (L, s, u) (L', s', u'). A \<turnstile>\<^sub>n \<langle>L, s, u\<rangle> \<rightarrow> \<langle>L', s', u'\<rangle>)
+          (\<lambda> (L, s, _). check_bexp \<phi> L s)
+    | formula.AG \<phi> \<Rightarrow>
+        Not o (\<lambda> (L, s, u). \<exists> L' s' u'. A \<turnstile>\<^sub>n \<langle>L, s, u\<rangle> \<rightarrow>* \<langle>L', s', u'\<rangle> \<and> \<not> check_bexp \<phi> L' s')
+    | formula.Leadsto \<phi> \<psi> \<Rightarrow>
+        Graph_Defs.leadsto
+          (\<lambda> (L, s, u) (L', s', u'). A \<turnstile>\<^sub>n \<langle>L, s, u\<rangle> \<rightarrow> \<langle>L', s', u'\<rangle>)
+          (\<lambda> (L, s, _). check_bexp \<phi> L s)
+          (\<lambda> (L, s, _). check_bexp \<psi> L s)
+    ) (L,s,u)
+    "
+proof -
+  have *:
+    "(Not \<circ>\<circ> case_prod) (\<lambda>L (s, _). check_bexp \<phi> L s) = (\<lambda> (L, s, _). \<not> check_bexp \<phi> L s)" for \<phi>
+    by auto
+  show ?thesis
+    unfolding models_def Graph_Defs.Alw_alw_iff Graph_Defs.Ex_alw_iff
+    by (cases "\<Phi>") (auto simp: * Ex_ev_eq_reachability[OF assms])
+qed
+
+context Reachability_Problem
+begin
+
+lemma init_dbm_reaches_iff:
+  "(\<exists> u \<in> [curry init_dbm]\<^bsub>v,n\<^esub>. \<exists> u'. conv_A A \<turnstile>' \<langle>l\<^sub>0, u\<rangle> \<rightarrow>* \<langle>l', u'\<rangle>)
+  \<longleftrightarrow> ([curry (init_dbm :: real DBM')]\<^bsub>v,n\<^esub> \<noteq> {} \<and>
+    (\<forall> u \<in> [curry init_dbm]\<^bsub>v,n\<^esub>. \<exists> u'. conv_A A \<turnstile>' \<langle>l\<^sub>0, u\<rangle> \<rightarrow>* \<langle>l', u'\<rangle>))
+  "
+  apply safe
+    apply force
+  subgoal for u1 u' u2
+    sorry
+  subgoal for u
+    by blast
+  done
+
+theorem reachable_decides_emptiness_new:
+  "(\<exists> D'. E\<^sup>*\<^sup>* a\<^sub>0 (l', D') \<and> [curry (conv_M D')]\<^bsub>v,n\<^esub> \<noteq> {})
+  \<longleftrightarrow> [curry (init_dbm :: real DBM')]\<^bsub>v,n\<^esub> \<noteq> {} \<and>
+    (\<forall> u \<in> [curry init_dbm]\<^bsub>v,n\<^esub>. \<exists> u'. conv_A A \<turnstile>' \<langle>l\<^sub>0, u\<rangle> \<rightarrow>* \<langle>l', u'\<rangle>)"
+  unfolding reachable_decides_emptiness init_dbm_reaches_iff ..
+
+lemma reachable_decides_emptiness'_new:
+  "(\<exists> D'. E\<^sup>*\<^sup>* a\<^sub>0 (l', D') \<and> [curry (conv_M D')]\<^bsub>v,n\<^esub> \<noteq> {})
+  \<longleftrightarrow> (\<forall> u. (\<forall> c \<in> {1..n}. u c = 0) \<longrightarrow> (\<exists> u'. conv_A A \<turnstile>' \<langle>l\<^sub>0, u\<rangle> \<rightarrow>* \<langle>l', u'\<rangle>))"
+  unfolding reachable_decides_emptiness_new
+  using init_dbm_semantics' init_dbm_semantics'' init_dbm_non_empty by blast
+
+lemma reachability_check_new_aux:
+  "(\<exists> D'. E\<^sup>*\<^sup>* a\<^sub>0 (l', D') \<and> [curry (conv_M D')]\<^bsub>v,n\<^esub> \<noteq> {} \<and> F l')
+  \<longleftrightarrow> (\<forall> u. (\<forall> c \<in> {1..n}. u c = 0) \<longrightarrow> (\<exists> u'. conv_A A \<turnstile>' \<langle>l\<^sub>0, u\<rangle> \<rightarrow>* \<langle>l', u'\<rangle> \<and> F l'))"
+  using reachable_decides_emptiness'_new[of l'] by fast
+
+theorem reachability_check_new:
+    "(\<exists> D'. E\<^sup>*\<^sup>* a\<^sub>0 (l', D') \<and> F_rel (l', D'))
+    \<longleftrightarrow> (\<forall> u. (\<forall> c \<in> {1..n}. u c = 0) \<longrightarrow> (\<exists> u'. conv_A A \<turnstile>' \<langle>l\<^sub>0, u\<rangle> \<rightarrow>* \<langle>l', u'\<rangle> \<and> F l'))"
+  using reachability_check_new_aux[of l'] check_diag_empty_spec reachable_empty_check_diag
+  unfolding F_rel_def by auto
+
+end
+
+
+context UPPAAL_Reachability_Problem_precompiled'
+begin
+
+(* XXX Fix naming problem *)
+(* XXX Unnecessary *)
+lemmas reachability_check_old =
+  Normalized_Zone_Semantics_Impl.Reachability_Problem.reachability_check
+  [OF Reachability_Problem_axioms]
+
+lemma F_reachable_correct'_new:
+  "impl.op.F_reachable
+  \<longleftrightarrow> (\<exists> L' s'. \<forall> u. (\<forall> c \<in> {1..m}. u c = 0) \<longrightarrow> (\<exists> u'.
+      conv_A A \<turnstile>' \<langle>(init, s\<^sub>0), u\<rangle> \<rightarrow>* \<langle>(L', s'), u'\<rangle>
+      \<and>  check_bexp \<phi> L' s')
+    )" if "formula = formula.EX \<phi>"
+  using that E_op''.E_from_op_reachability_check reachability_check_new
+  unfolding impl.E_op_F_reachable E_op''.F_reachable_def E_op''.reachable_def
+  unfolding F_def by auto
+
+lemma F_reachable_correct'_new':
+  "impl.op.F_reachable
+  \<longleftrightarrow> (\<exists> L' s'. \<forall> u. (\<forall> c \<in> {1..m}. u c = 0) \<longrightarrow> (\<exists> u'.
+      conv_A A \<turnstile>' \<langle>(init, s\<^sub>0), u\<rangle> \<rightarrow>* \<langle>(L', s'), u'\<rangle>
+      \<and>  \<not> check_bexp \<phi> L' s')
+    )" if "formula = formula.AG \<phi>"
+  using that E_op''.E_from_op_reachability_check reachability_check_new
+  unfolding impl.E_op_F_reachable E_op''.F_reachable_def E_op''.reachable_def
+  unfolding F_def by auto
+
+lemma F_reachable_correct_new:
+  "impl.op.F_reachable
+  \<longleftrightarrow> (\<exists> L' s'. \<forall> u. (\<forall> c \<in> {1..m}. u c = 0) \<longrightarrow> (\<exists> u'.
+      conv N \<turnstile>\<^sub>max_steps \<langle>init, s\<^sub>0, u\<rangle> \<rightarrow>* \<langle>L', s', u'\<rangle>
+       \<and> check_bexp \<phi> L' s')
+    )" if "formula = formula.EX \<phi>" "start_inv_check"
+    unfolding F_reachable_correct'_new[OF that(1)]
+    apply (subst product'.prod_correct[symmetric])
+    using prod_conv p_p p_gt_0 apply simp
+    using prod_conv p_p p_gt_0 apply simp
+    using F_reachable_equiv[OF that(2)]
+    apply (simp add: F_def)
+      apply (simp add: that(1))
+    sorry
+    (* by (simp add: F_def, simp add: that(1)) *)
+
+lemma F_reachable_correct_new':
+  "impl.op.F_reachable
+  \<longleftrightarrow> (\<exists> L' s'. \<forall> u. (\<forall> c \<in> {1..m}. u c = 0) \<longrightarrow> (\<exists> u'.
+      conv N \<turnstile>\<^sub>max_steps \<langle>init, s\<^sub>0, u\<rangle> \<rightarrow>* \<langle>L', s', u'\<rangle>
+       \<and> \<not> check_bexp \<phi> L' s')
+    )" if "formula = formula.AG \<phi>" "start_inv_check"
+    unfolding F_reachable_correct'_new'[OF that(1)]
+    apply (subst product'.prod_correct[symmetric])
+    using prod_conv p_p p_gt_0 apply simp
+    using prod_conv p_p p_gt_0 apply simp
+    using F_reachable_equiv[OF that(2)]
+    apply (simp add: F_def)
+      apply (simp add: that(1))
+    sorry
+
+thm reachability_checker'_def impl.pw_impl_hnr_F_reachable
+
+thm final_fun_def F_def
+
+thm
+  impl.leadsto_impl_hnr[OF _]
+  impl.Alw_ev_impl_hnr[OF _]
+
+term formula term pw_impl
+
+definition
+  "Alw_ev_checker = dfs_map_impl' TYPE('bb) TYPE('cc) TYPE('dd)
+     (impl.succs_P_impl' final_fun) impl.a\<^sub>0_impl impl.subsumes_impl (return \<circ> fst)
+     impl.state_copy_impl"
+
+definition
+  "leadsto_checker \<psi> = do {
+      r \<leftarrow> leadsto_impl TYPE('bb) TYPE('cc) TYPE('dd)
+      impl.state_copy_impl (impl.succs_P_impl' (\<lambda> (L, s). \<not> check_bexp \<psi> L s))
+      impl.a\<^sub>0_impl impl.subsumes_impl (return \<circ> fst)
+      impl.succs_impl' impl.emptiness_check_impl impl.F_impl
+      (impl.Q_impl (\<lambda> (L, s). \<not> check_bexp \<psi> L s));
+      return (\<not> r)
+    }"
+
+definition
+  "model_checker = (
+  case formula of
+    formula.EX _ \<Rightarrow> reachability_checker' |
+    formula.AG _ \<Rightarrow> do {
+      r \<leftarrow> reachability_checker';
+      return (\<not> r)
+    } |
+    formula.AX _ \<Rightarrow> do {
+      r \<leftarrow> if PR_CONST (\<lambda>(x, y). F x y) (init, s\<^sub>0)
+      then Alw_ev_checker TYPE('bb) TYPE('cc) TYPE('dd)
+      else return False;
+      return (\<not> r)
+    } |
+    formula.EG _ \<Rightarrow>
+      if PR_CONST (\<lambda>(x, y). F x y) (init, s\<^sub>0)
+      then Alw_ev_checker TYPE('bb) TYPE('cc) TYPE('dd)
+      else return False |
+    formula.Leadsto _ \<psi> \<Rightarrow> leadsto_checker TYPE('bb) TYPE('cc) TYPE('dd) \<psi>
+  )
+  "
+
+term model_checker
+
+thm model_checker_def
+
+term TA.steps
+
+sublocale sem: Graph_Defs "\<lambda> (l, u) (l', u'). conv_A A \<turnstile> \<langle>l, u\<rangle> \<rightarrow> \<langle>l', u'\<rangle>" .
+
+term "conv N"
+
+sublocale network: Graph_Defs "\<lambda> (L, s, u) (L', s', u'). conv N \<turnstile>\<^sub>n \<langle>L, s, u\<rangle> \<rightarrow> \<langle>L', s', u'\<rangle>" .
+
+term a\<^sub>0
+
+lemma models_correct:
+  "conv N,(init, s\<^sub>0, u\<^sub>0) \<Turnstile>\<^sub>max_steps \<Phi> = (case \<Phi> of
+    formula.EX \<phi> \<Rightarrow>
+        (\<lambda> ((L, s), u). \<exists> L' s' u'. conv_A A \<turnstile>' \<langle>(L, s), u\<rangle> \<rightarrow>* \<langle>(L', s'), u'\<rangle> \<and> check_bexp \<phi> L' s')
+  | formula.EG \<phi> \<Rightarrow>
+      Not o Graph_Defs.Alw_ev
+        (\<lambda> (l, u) (l', u'). conv_A A \<turnstile>' \<langle>l, u\<rangle> \<rightarrow> \<langle>l', u'\<rangle>)
+        (\<lambda> ((L, s), _). \<not> check_bexp \<phi> L s)
+  | formula.AX \<phi> \<Rightarrow>
+      Graph_Defs.Alw_ev
+        (\<lambda> (l, u) (l', u'). conv_A A \<turnstile>' \<langle>l, u\<rangle> \<rightarrow> \<langle>l', u'\<rangle>)
+        (\<lambda> ((L, s), _). check_bexp \<phi> L s)
+  | formula.AG \<phi> \<Rightarrow>
+      Not o (\<lambda> ((L, s), u).
+        \<exists> L' s' u'. conv_A A \<turnstile>' \<langle>(L, s), u\<rangle> \<rightarrow>* \<langle>(L', s'), u'\<rangle> \<and> \<not> check_bexp \<phi> L' s'
+      )
+  | formula.Leadsto \<phi> \<psi> \<Rightarrow>
+      Graph_Defs.leadsto
+        (\<lambda> (l, u) (l', u'). conv_A A \<turnstile>' \<langle>l, u\<rangle> \<rightarrow> \<langle>l', u'\<rangle>)
+        (\<lambda> ((L, s), _). check_bexp \<phi> L s)
+        (\<lambda> ((L, s), _). check_bexp \<psi> L s)
+  ) ((init, s\<^sub>0), u\<^sub>0)" if start_inv_check "\<forall> c \<in> {1..m}. u\<^sub>0 c = 0"
+proof -
+  interpret start: Reachability_Problem_start "(init, s\<^sub>0)" "PR_CONST (\<lambda> (l, s). F l s)" m A k_fun
+    apply standard
+    using that(1) unfolding start_inv_check .
+  have "u\<^sub>0 \<turnstile> inv_of (conv_A A) (init, s\<^sub>0)"
+    using start.start_vals[OF that(2)] .
+  show ?thesis
+    apply (subst models_alt_def)
+    subgoal
+      sorry
+    subgoal
+      sorry
+    subgoal
+      by blast
+     apply (cases \<Phi>)
+  using [[goals_limit=1]]
+    subgoal for \<phi>
+    using prod_conv p_p p_gt_0
+      steps_steps'_equiv[of _ \<open>conv_A A\<close> "(init, s\<^sub>0)", OF start.start_vals[OF that(2)]]
+    by (fastforce simp: product'.prod_correct[symmetric, simplified])
+  sorry
+qed
+
+(* XXX *)
+lemma init_state_in_state_set:
+  "(init, s\<^sub>0) \<in> Normalized_Zone_Semantics_Impl_Refine.state_set (trans_of A)"
+  sorry
+
+(* XXX Remove less general versions *)
+lemma final_fun_final':
+  "((\<lambda> (L, s). P L s), (\<lambda> (L, s). P L s)) \<in> inv_rel states'" for P
+  unfolding F_def final_fun_def inv_rel_def in_set_member[symmetric] list_ex_iff
+  by (force dest!: states'_states')
+
+lemma final_fun_final[intro, simp]:
+  "((\<lambda> (L, s). P L s), (\<lambda> (L, s). P L s)) \<in> inv_rel states" for P
+  using final_fun_final' states_states' by (rule inv_rel_mono)
+
+term "conv N,(init, s\<^sub>0, u\<^sub>0) \<Turnstile>\<^sub>max_steps formula"
+
+lemma hn_refine_emp_neg_RES:
+  assumes "hn_refine emp (f) emp bool_assn (RES Y)"
+  shows "hn_refine emp (do {r \<leftarrow> f; return (\<not> r)}) emp bool_assn (RES {\<not> x | x. x \<in> Y})"
+  using assms[unfolded hn_refine_def]
+  by sepref_to_hoare sep_auto
+
+lemma hfref_emp_neg_RES:
+  assumes "(uncurry0 f, uncurry0 (RES Y)) \<in> (unit_assn, unit_assn) \<rightarrow>\<^sub>a bool_assn"
+  shows "(uncurry0 (do {r \<leftarrow> f; return (\<not> r)}), uncurry0 (RES {\<not> x | x. x \<in> Y}))
+  \<in> (unit_assn, unit_assn) \<rightarrow>\<^sub>a bool_assn"
+  using assms[to_hnr]
+  by (auto intro!: hfrefI hn_refine_emp_neg_RES simp: pure_unit_rel_eq_empty)
+
+lemma hn_refine_emp_return_neg_RES:
+  assumes "hn_refine emp (return False) emp bool_assn (RES Y)"
+  shows "hn_refine emp (return True) emp bool_assn (RES {\<not> x | x. x \<in> Y})"
+  using hn_refine_emp_neg_RES[OF assms] by simp
+
+lemma Alw_ev_bisim:
+  "(\<exists>u\<^sub>0. (\<forall>c\<in>{Suc 0..m}. u\<^sub>0 c = 0) \<and>
+                  \<not> Alw_ev (\<lambda>((L, s), _). \<not> check_bexp \<phi> L s) ((init, s\<^sub>0), u\<^sub>0))
+  = (\<forall>u\<^sub>0. (\<forall>c\<in>{Suc 0..m}. u\<^sub>0 c = 0) \<longrightarrow>
+               \<not> Alw_ev (\<lambda>((L, s), _). \<not> check_bexp \<phi> L s) ((init, s\<^sub>0), u\<^sub>0))"
+  sorry
+
+lemma maxiscope_impl:
+  "(\<forall> a. P a \<longrightarrow> (\<forall> b. Q a b)) = (\<forall> b a. P a \<longrightarrow> Q a b)" for P Q
+  by auto
+
+thm reachability_checker'_def model_checker_def
+
+theorem reachability_check':
+  "(uncurry0 (model_checker TYPE('bb) TYPE('cc) TYPE('dd)),
+    uncurry0 (
+      Refine_Basic.RETURN (
+        \<forall> u\<^sub>0. (\<forall> c \<in> {1..m}. u\<^sub>0 c = 0) \<longrightarrow> conv N,(init, s\<^sub>0, u\<^sub>0) \<Turnstile>\<^sub>max_steps formula
+      )
+    )
+   )
+  \<in> unit_assn\<^sup>k \<rightarrow>\<^sub>a bool_assn"
+  if start_inv_check "\<forall>u\<^sub>0. (\<forall>c\<in>{1..m}. u\<^sub>0 c = 0) \<longrightarrow> \<not> deadlock ((init, s\<^sub>0), u\<^sub>0)"
+proof -
+  have *: "(\<lambda>(l, u). \<not> (case l of (L, s) \<Rightarrow> (Not \<circ>\<circ>\<circ> check_bexp) \<phi> L s))
+    = (\<lambda>((L, s), _). check_bexp \<phi> L s)" for \<phi>
+    by auto
+  have **:
+    "(\<lambda>(l, u). \<not> (case l of (L, s) \<Rightarrow> check_bexp \<phi> L s)) = (\<lambda>((L, s), _). \<not> check_bexp \<phi> L s)"
+    for \<phi> by auto
+  have ***:
+    "(\<lambda>(l, u). case l of (L, s) \<Rightarrow> check_bexp \<phi> L s) = (\<lambda>((L, s), _). check_bexp \<phi> L s)" for \<phi>
+    by auto
+  have ****: "{\<not> xa |xa. (\<not> xa) = x} = {x}" for x
+    by auto
+
+  show ?thesis
+    using models_correct[OF \<open>start_inv_check\<close>]
+    apply simp
+    unfolding model_checker_def reachability_checker'_def Alw_ev_checker_def leadsto_checker_def
+    apply (cases formula; simp)
+
+      -- \<open>\<open>EX\<close>\<close>
+    subgoal premises prems for \<phi>
+      using impl.pw_impl_hnr_F_reachable
+      apply (subst (asm) F_reachable_correct_new)
+        apply (rule prems; fail)
+       apply (rule that; fail)
+      apply auto
+      sorry
+
+        -- \<open>\<open>EG\<close>\<close>
+    subgoal premises prems for \<phi>
+      using impl.Alw_ev_impl_hnr[OF init_state_in_state_set, where 'bb = 'bb and 'cc = 'cc and 'dd = 'dd]
+      unfolding final_fun_def F_def
+      unfolding
+        UPPAAL_Reachability_Problem_precompiled'.final_fun_def[
+          OF UPPAAL_Reachability_Problem_precompiled'_axioms
+          ]
+        UPPAAL_Reachability_Problem_precompiled_defs.F_def
+      unfolding prems(2)
+      apply simp
+      unfolding Refine_Basic.RETURN_def **
+      by (auto simp add: pure_unit_rel_eq_empty Alw_ev_bisim intro: hn_refine_ref hfrefI)
+
+        -- \<open>\<open>AX\<close>\<close>
+    subgoal premises prems for \<phi>
+      using impl.Alw_ev_impl_hnr[OF init_state_in_state_set, where 'bb = 'bb and 'cc = 'cc and 'dd = 'dd]
+      unfolding final_fun_def F_def
+      unfolding UPPAAL_Reachability_Problem_precompiled_defs.F_def
+      apply (subst
+          UPPAAL_Reachability_Problem_precompiled'.final_fun_def[
+            OF UPPAAL_Reachability_Problem_precompiled'_axioms
+            ])
+      apply (safe; clarsimp simp: prems(2))
+      subgoal premises prems
+        using prems(1)[unfolded *, THEN hfref_emp_neg_RES]
+        by (simp add: RETURN_def disj_not1[symmetric])
+      subgoal premises prems
+        using prems(1)[unfolded *, THEN hfref_emp_neg_RES]
+        by (simp add: RETURN_def disj_not1[symmetric])
+      done
+
+        -- \<open>\<open>AG\<close>\<close>
+    subgoal premises prems for \<phi>
+      using impl.pw_impl_hnr_F_reachable
+      apply (subst (asm) F_reachable_correct_new')
+        apply (rule prems; fail)
+       apply (rule that; fail)
+      apply auto
+      subgoal premises prems
+        using prems(1)[unfolded * RETURN_def, THEN hfref_emp_neg_RES]
+        apply (simp add: RETURN_def)
+        apply (simp only: maxiscope_impl)
+          -- "We also need bisimilarity here."
+        sorry
+      done
+
+        -- \<open>\<open>Leadsto\<close>\<close>
+    subgoal premises prems for \<phi> \<psi>
+      using impl.leadsto_impl_hnr[
+          OF final_fun_final init_state_in_state_set that(2), of "Not oo check_bexp \<psi>"
+          ]
+      unfolding * F_def
+      by (auto simp: prems(2) RETURN_def *** **** dest: hfref_emp_neg_RES)
+    done
+qed
+
+term A
+
+thm dfs_map_impl'_def
+
+thm
+  impl.leadsto_impl_hnr[OF _ init_state_in_state_set]
+  impl.Alw_ev_impl_hnr[OF init_state_in_state_set]
+
+term E thm E_def thm start_inv_check_def
+
+thm reachability_checker'_def Alw_ev_checker_def leadsto_checker_def
+
+lemma Alw_ev_checker_alt_def':
+  "Alw_ev_checker TYPE('bb) TYPE('cc) TYPE('dd) \<equiv>
+    let
+      key = return \<circ> fst;
+      sub = impl.subsumes_impl;
+      copy = impl.state_copy_impl;
+      start = impl.a\<^sub>0_impl;
+      succs =  impl.succs_P_impl' final_fun
+    in dfs_map_impl' TYPE('bb) TYPE('cc) TYPE('dd) succs start sub key copy"
+  unfolding Alw_ev_checker_def by simp
+
+lemma leadsto_checker_alt_def':
+  "leadsto_checker TYPE('bb) TYPE('cc) TYPE('dd) \<psi> \<equiv>
+    let
+      key = return \<circ> fst;
+      sub = impl.subsumes_impl;
+      copy = impl.state_copy_impl;
+      start = impl.a\<^sub>0_impl;
+      final = impl.F_impl;
+      final' = (impl.Q_impl (\<lambda>(L, s). \<not> check_bexp \<psi> L s));
+      succs =  impl.succs_P_impl' (\<lambda>(L, s). \<not> check_bexp \<psi> L s);
+      succs' =  impl.succs_impl';
+      empty = impl.emptiness_check_impl
+    in do {
+      r \<leftarrow>
+      leadsto_impl TYPE('bb) TYPE('cc) TYPE('dd) copy succs start sub key succs' empty final final';
+      return (\<not> r)
+    }"
+  unfolding leadsto_checker_def by simp
+
+schematic_goal succs_P_impl_alt_def:
+  "impl.succs_P_impl (\<lambda>(L, s). P L s) \<equiv> ?impl" for P
+  unfolding impl.succs_P_impl_def[OF final_fun_final]
+  unfolding k_impl_alt_def
+  apply (tactic
+      \<open>pull_tac
+      @{term
+        "\<lambda> (l, _). IArray (map (\<lambda> c. Max {k_i !! i !! (l ! i) !! c | i. i \<in> {0..<p}}) [0..<m+1])"
+      }
+      @{context}
+     \<close>
+      )
+  apply (tactic \<open>pull_tac @{term "inv_fun"} @{context}\<close>)
+  apply (tactic \<open>pull_tac @{term "trans_fun"} @{context}\<close>)
+  unfolding inv_fun_def[abs_def] trans_fun_def[abs_def] trans_s_fun_def trans_i_fun_def trans_i_from_def
+  apply (tactic \<open>pull_tac @{term "IArray (map IArray inv)"} @{context}\<close>)
+  apply (tactic \<open>pull_tac @{term "IArray (map IArray trans_out_map)"} @{context}\<close>)
+  apply (tactic \<open>pull_tac @{term "IArray (map IArray trans_in_map)"} @{context}\<close>)
+  apply (tactic \<open>pull_tac @{term "IArray (map IArray trans_i_map)"} @{context}\<close>)
+  by (rule Pure.reflexive)
+
+(* XXX These implementations contain unnecessary list reversals *)
+lemmas succs_P'_impl_alt_def =
+  impl.succs_P_impl'_def[OF final_fun_final, unfolded succs_P_impl_alt_def]
+
+lemmas succs_impl'_alt_def =
+  impl.succs_impl'_def[unfolded succs_impl_alt_def]
+
+lemma reachability_checker'_alt_def':
+  "reachability_checker' \<equiv>
+    do {
+      let key = return \<circ> fst;
+      let sub = impl.subsumes_impl;
+      let copy = impl.state_copy_impl;
+      let start = impl.a\<^sub>0_impl;
+      let final = impl.F_impl;
+      let succs =  impl.succs_impl;
+      let empty = impl.emptiness_check_impl;
+      x \<leftarrow> pw_impl key copy sub start final succs empty;
+      return x
+    }"
+  unfolding reachability_checker'_def by simp
+
+schematic_goal reachability_checker'_alt_def:
+  "reachability_checker' \<equiv> ?impl"
+  unfolding reachability_checker'_alt_def' impl.succs_impl_def
+  unfolding impl.E_op''_impl_def impl.abstr_repair_impl_def impl.abstra_repair_impl_def
+  unfolding
+    impl.start_inv_check_impl_def impl.unbounded_dbm_impl_def
+    impl.unbounded_dbm'_def unbounded_dbm_def
+  unfolding k_impl_alt_def
+  apply (tactic \<open>pull_tac @{term k_i} @{context}\<close>)
+  apply (tactic \<open>pull_tac @{term "inv_fun"} @{context}\<close>) (* XXX This is not pulling anything *)
+  apply (tactic \<open>pull_tac @{term "trans_fun"} @{context}\<close>)
+  unfolding impl.init_dbm_impl_def impl.a\<^sub>0_impl_def
+  unfolding impl.F_impl_def
+  unfolding final_fun_def[abs_def]
+  unfolding impl.subsumes_impl_def
+  unfolding impl.emptiness_check_impl_def
+  unfolding impl.state_copy_impl_def
+  by (rule Pure.reflexive)
+
+schematic_goal Alw_ev_checker_alt_def:
+  "Alw_ev_checker TYPE('bb) TYPE('cc) TYPE('dd) \<equiv> ?impl"
+  unfolding Alw_ev_checker_alt_def' final_fun_def
+    impl.succs_P_impl_def[OF final_fun_final] impl.succs_P_impl'_def[OF final_fun_final]
+  unfolding impl.E_op''_impl_def impl.abstr_repair_impl_def impl.abstra_repair_impl_def
+  unfolding
+    impl.start_inv_check_impl_def impl.unbounded_dbm_impl_def
+    impl.unbounded_dbm'_def unbounded_dbm_def
+  unfolding k_impl_alt_def
+  apply (tactic \<open>pull_tac @{term k_i} @{context}\<close>)
+  apply (tactic \<open>pull_tac @{term "inv_fun"} @{context}\<close>) (* XXX This is not pulling anything *)
+  apply (tactic \<open>pull_tac @{term "trans_fun"} @{context}\<close>)
+  unfolding impl.init_dbm_impl_def impl.a\<^sub>0_impl_def
+  unfolding impl.F_impl_def
+  unfolding final_fun_def[abs_def]
+  unfolding impl.subsumes_impl_def
+  unfolding impl.emptiness_check_impl_def
+  unfolding impl.state_copy_impl_def
+  by (rule Pure.reflexive)
+
+schematic_goal leadsto_checker_alt_def:
+  "leadsto_checker TYPE('bb) TYPE('cc) TYPE('dd) \<equiv> ?impl"
+  unfolding leadsto_checker_alt_def'
+  unfolding impl.F_impl_def impl.Q_impl_def[OF final_fun_final]
+  unfolding impl.succs_P_impl'_def[OF final_fun_final]
+  unfolding impl.succs_impl'_def impl.succs_impl_def impl.succs_P_impl_def[OF final_fun_final]
+  unfolding impl.E_op''_impl_def impl.abstr_repair_impl_def impl.abstra_repair_impl_def
+  unfolding
+    impl.start_inv_check_impl_def impl.unbounded_dbm_impl_def
+    impl.unbounded_dbm'_def unbounded_dbm_def
+  unfolding k_impl_alt_def
+  apply (tactic \<open>pull_tac @{term k_i} @{context}\<close>)
+  apply (tactic \<open>pull_tac @{term "inv_fun"} @{context}\<close>) (* XXX This is not pulling anything *)
+  apply (tactic \<open>pull_tac @{term "trans_fun"} @{context}\<close>)
+  unfolding impl.init_dbm_impl_def impl.a\<^sub>0_impl_def
+  unfolding final_fun_def
+  unfolding impl.subsumes_impl_def
+  unfolding impl.emptiness_check_impl_def
+  unfolding impl.state_copy_impl_def
+  by (rule Pure.reflexive)
+
+thm model_checker_def[unfolded
+  reachability_checker'_alt_def Alw_ev_checker_alt_def leadsto_checker_alt_def
+]
+
+schematic_goal reachability_checker'_alt_def_refined:
+  "reachability_checker' \<equiv> ?impl"
+  unfolding reachability_checker'_alt_def
+  unfolding fw_impl'_int
+  unfolding inv_fun_def trans_fun_def trans_s_fun_def trans_i_fun_def
+  unfolding trans_i_from_impl
+  unfolding runf_impl runt_impl check_g_impl pairs_by_action_impl check_pred_impl
+  apply (tactic \<open>pull_tac @{term "IArray (map IArray inv)"} @{context}\<close>)
+  apply (tactic \<open>pull_tac @{term "IArray (map IArray trans_out_map)"} @{context}\<close>)
+  apply (tactic \<open>pull_tac @{term "IArray (map IArray trans_in_map)"} @{context}\<close>)
+  apply (tactic \<open>pull_tac @{term "IArray (map IArray trans_i_map)"} @{context}\<close>)
+  apply (tactic \<open>pull_tac @{term "IArray bounds"} @{context}\<close>)
+  apply (tactic \<open>pull_tac @{term PF} @{context}\<close>)
+  apply (tactic \<open>pull_tac @{term PT} @{context}\<close>)
+  unfolding PF_alt_def PT_alt_def
+  apply (tactic \<open>pull_tac @{term PROG'} @{context}\<close>)
+  unfolding PROG'_def
+  apply (tactic \<open>pull_tac @{term "length prog"} @{context}\<close>)
+  apply (tactic \<open>pull_tac @{term "IArray (map (map_option stripf) prog)"} @{context}\<close>)
+  apply (tactic \<open>pull_tac @{term "IArray (map (map_option stript) prog)"} @{context}\<close>)
+  apply (tactic \<open>pull_tac @{term "IArray prog"} @{context}\<close>)
+  unfolding all_actions_by_state_impl
+  apply (tactic \<open>pull_tac @{term "[0..<p]"} @{context}\<close>)
+  apply (tactic \<open>pull_tac @{term "[0..<na]"} @{context}\<close>)
+  apply (tactic \<open>pull_tac @{term "{0..<p}"} @{context}\<close>)
+  apply (tactic \<open>pull_tac @{term "[0..<m+1]"} @{context}\<close>)
+  by (rule Pure.reflexive)
+
+schematic_goal Alw_ev_checker_alt_def_refined:
+  "Alw_ev_checker TYPE('bb) TYPE('cc) TYPE('dd) \<equiv> ?impl"
+  unfolding Alw_ev_checker_alt_def
+  unfolding fw_impl'_int
+  unfolding inv_fun_def trans_fun_def trans_s_fun_def trans_i_fun_def
+  unfolding trans_i_from_impl
+  unfolding runf_impl runt_impl check_g_impl pairs_by_action_impl check_pred_impl
+  apply (tactic \<open>pull_tac @{term "IArray (map IArray inv)"} @{context}\<close>)
+  apply (tactic \<open>pull_tac @{term "IArray (map IArray trans_out_map)"} @{context}\<close>)
+  apply (tactic \<open>pull_tac @{term "IArray (map IArray trans_in_map)"} @{context}\<close>)
+  apply (tactic \<open>pull_tac @{term "IArray (map IArray trans_i_map)"} @{context}\<close>)
+  apply (tactic \<open>pull_tac @{term "IArray bounds"} @{context}\<close>)
+  apply (tactic \<open>pull_tac @{term PF} @{context}\<close>)
+  apply (tactic \<open>pull_tac @{term PT} @{context}\<close>)
+  unfolding PF_alt_def PT_alt_def
+  apply (tactic \<open>pull_tac @{term PROG'} @{context}\<close>)
+  unfolding PROG'_def
+  apply (tactic \<open>pull_tac @{term "length prog"} @{context}\<close>)
+  apply (tactic \<open>pull_tac @{term "IArray (map (map_option stripf) prog)"} @{context}\<close>)
+  apply (tactic \<open>pull_tac @{term "IArray (map (map_option stript) prog)"} @{context}\<close>)
+  apply (tactic \<open>pull_tac @{term "IArray prog"} @{context}\<close>)
+  unfolding all_actions_by_state_impl
+  apply (tactic \<open>pull_tac @{term "[0..<p]"} @{context}\<close>)
+  apply (tactic \<open>pull_tac @{term "[0..<na]"} @{context}\<close>)
+  apply (tactic \<open>pull_tac @{term "{0..<p}"} @{context}\<close>)
+  apply (tactic \<open>pull_tac @{term "[0..<m+1]"} @{context}\<close>)
+  by (rule Pure.reflexive)
+
+schematic_goal leadsto_checker_alt_def_refined:
+  "leadsto_checker TYPE('bb) TYPE('cc) TYPE('dd) \<equiv> ?impl"
+  unfolding leadsto_checker_alt_def
+  unfolding fw_impl'_int
+  unfolding inv_fun_def trans_fun_def trans_s_fun_def trans_i_fun_def
+  unfolding trans_i_from_impl
+  unfolding runf_impl runt_impl check_g_impl pairs_by_action_impl check_pred_impl
+  apply (tactic \<open>pull_tac @{term "IArray (map IArray inv)"} @{context}\<close>)
+  apply (tactic \<open>pull_tac @{term "IArray (map IArray trans_out_map)"} @{context}\<close>)
+  apply (tactic \<open>pull_tac @{term "IArray (map IArray trans_in_map)"} @{context}\<close>)
+  apply (tactic \<open>pull_tac @{term "IArray (map IArray trans_i_map)"} @{context}\<close>)
+  apply (tactic \<open>pull_tac @{term "IArray bounds"} @{context}\<close>)
+  apply (tactic \<open>pull_tac @{term PF} @{context}\<close>)
+  apply (tactic \<open>pull_tac @{term PT} @{context}\<close>)
+  unfolding PF_alt_def PT_alt_def
+  apply (tactic \<open>pull_tac @{term PROG'} @{context}\<close>)
+  unfolding PROG'_def
+  apply (tactic \<open>pull_tac @{term "length prog"} @{context}\<close>)
+  apply (tactic \<open>pull_tac @{term "IArray (map (map_option stripf) prog)"} @{context}\<close>)
+  apply (tactic \<open>pull_tac @{term "IArray (map (map_option stript) prog)"} @{context}\<close>)
+  apply (tactic \<open>pull_tac @{term "IArray prog"} @{context}\<close>)
+  unfolding all_actions_by_state_impl
+  apply (tactic \<open>pull_tac @{term "[0..<p]"} @{context}\<close>)
+  apply (tactic \<open>pull_tac @{term "[0..<na]"} @{context}\<close>)
+  apply (tactic \<open>pull_tac @{term "{0..<p}"} @{context}\<close>)
+  apply (tactic \<open>pull_tac @{term "[0..<m+1]"} @{context}\<close>)
+  by (rule Pure.reflexive)
+
+end
+
+concrete_definition reachability_checker'
+  uses UPPAAL_Reachability_Problem_precompiled'.reachability_checker'_alt_def_refined
+
+concrete_definition Alw_ev_checker
+  uses UPPAAL_Reachability_Problem_precompiled'.Alw_ev_checker_alt_def_refined
+
+concrete_definition leadsto_checker
+  uses UPPAAL_Reachability_Problem_precompiled'.leadsto_checker_alt_def_refined
+
+thm reachability_checker'_def Alw_ev_checker_def leadsto_checker_def
+
+context UPPAAL_Reachability_Problem_precompiled'
+begin
+
+lemmas model_checker_def_refined = model_checker_def[unfolded
+    reachability_checker'.refine[OF UPPAAL_Reachability_Problem_precompiled'_axioms]
+    Alw_ev_checker.refine[OF UPPAAL_Reachability_Problem_precompiled'_axioms]
+    leadsto_checker.refine[OF UPPAAL_Reachability_Problem_precompiled'_axioms]
+  ]
+
+thm model_checker_def_refined
+
+end
+
+concrete_definition model_checker uses
+  UPPAAL_Reachability_Problem_precompiled'.model_checker_def_refined
+
+definition [code]:
+  "precond_mc p m k max_steps I T prog final bounds P s\<^sub>0 na \<equiv>
+    if UPPAAL_Reachability_Problem_precompiled' p m max_steps I T prog bounds P s\<^sub>0 na k
+    then
+      model_checker TYPE('bb) TYPE('cc) TYPE('dd) p m max_steps I T prog bounds P s\<^sub>0 na k final
+      \<bind> (\<lambda> x. return (Some x))
+    else return None"
+
+prepare_code_thms dfs_map_impl'_def leadsto_impl_def
+
+(* XXX Debug code generator performance problems in conjunction with Let-expressions *)
+lemmas [code] =
+  reachability_checker'_def[unfolded Let_def]
+  Alw_ev_checker_def[unfolded Let_def]
+  leadsto_checker_def[unfolded Let_def]
+  model_checker_def[unfolded UPPAAL_Reachability_Problem_precompiled_defs.F_def PR_CONST_def]
+
+export_code
+  reachability_checker'
+  checking SML_imp
+
+export_code open
+  Alw_ev_checker
+  checking SML_imp
+
+export_code open
+  leadsto_checker
+  checking SML_imp
+
+export_code open
+  model_checker
+  checking SML_imp
+
+export_code
+  precond_mc Pure.type init_pred_check time_indep_check1 time_indep_check1 conjunction_check2
+  checking SML_imp
+
+end (* Theory *)
